src/program_proof/memkv/memkv_marshal_get_proof.v
@@ -1,0 +1,75 @@
+From Perennial.program_proof Require Import proof_prelude.
+From Goose.github_com.mit_pdos.gokv Require Import memkv.
+From Perennial.goose_lang Require Import ffi.grove_ffi.
+
+(*
+  Defines Coq request and reply types for shard server Get RPC. Also defines
+  has_encoding for Get Request/Reply and provides WPs for {de|en}codeGetRe{ply|quest}()
+ *)
+
+Section memkv_marshal_get_proof.
+
+Context `{!heapG Σ}.
+
+Record GetRequestC := mkGetRequestC {
+  GR_CID : u64;
+  GR_Seq : u64;
+  GR_Key : u64
+}.
+
+Record GetReplyC := mkGetReplyC {
+  GR_Err : u64;
+  GR_Value : list u8
+}.
+
+Definition own_GetRequest args_ptr args : iProp Σ :=
+  "HCID" ∷ args_ptr ↦[GetRequest.S :: "CID"] #args.(GR_CID) ∗
+  "HSeq" ∷ args_ptr ↦[GetRequest.S :: "Seq"] #args.(GR_Seq) ∗
+  "HKey" ∷ args_ptr ↦[GetRequest.S :: "Key"] #args.(GR_Key)
+.
+
+Definition own_GetReply reply_ptr rep : iProp Σ :=
+  ∃ val_sl,
+  "HErr" ∷ reply_ptr ↦[GetReply.S :: "Err"] #rep.(GR_Err) ∗
+  "HValue" ∷ reply_ptr ↦[GetReply.S :: "Value"] (slice_val val_sl) ∗
+  "HValue_sl" ∷ typed_slice.is_slice val_sl byteT 1%Qp rep.(GR_Value)
+.
+
+Axiom has_encoding_GetRequest : (list u8) → GetRequestC → Prop.
+Axiom has_encoding_GetReply : (list u8) → GetReplyC → Prop.
+
+Lemma wp_encodeGetRequest (cid seq key:u64) :
+  {{{
+       True
+  }}}
+    encodeGetRequest (#cid, (#seq, (#key, #())))%V
+  {{{
+       (reqData:list u8) req_sl, RET (slice_val req_sl); ⌜has_encoding_GetRequest reqData {| GR_CID:=cid; GR_Seq:=seq; GR_Key:=key |}⌝ ∗
+                                               typed_slice.is_slice req_sl byteT 1%Qp reqData
+  }}}.
+Proof.
+Admitted.
+
+Lemma has_encoding_GetRequest_inj (reqRaw:list u8) req req' :
+  has_encoding_GetRequest reqRaw req →
+  has_encoding_GetRequest reqRaw req' →
+  req = req'.
+Proof.
+Admitted.
+
+Lemma wp_decodeGetReply rep rep_sl repData :
+  {{{
+       typed_slice.is_slice rep_sl byteT 1%Qp repData ∗
+       ⌜has_encoding_GetReply repData rep ⌝
+  }}}
+    decodeGetReply (slice_val rep_sl)
+  {{{
+       (rep_ptr:loc) val_sl, RET #rep_ptr;
+       rep_ptr ↦[GetReply.S :: "Err"] #rep.(GR_Err) ∗
+       rep_ptr ↦[GetReply.S :: "Value"] (slice_val val_sl) ∗
+       typed_slice.is_slice val_sl byteT 1%Qp rep.(GR_Value)
+  }}}.
+Proof.
+Admitted.
+
+End memkv_marshal_get_proof.
